Added WG8 and BV lemmas

src/CongruenceScript.sml
@@ -437,7 +437,7 @@ Proof
  >> BETA_TAC >> art []
 QED
 
-Theorem NOT_WG0 :
+Theorem NO_WG0 :
     ~WG (\t. t)
 Proof
     ONCE_REWRITE_TAC [WG_cases] >> rpt STRIP_TAC (* 6 subgoals *)
@@ -446,6 +446,34 @@ Proof
  >> fs [FUN_EQ_THM]
  >> Q.PAT_X_ASSUM `!t. t = X` (ASSUME_TAC o (Q.SPEC `nil`))
  >> fs [CCS_distinct]
+QED
+
+Definition CCS_const_def :
+    CCS_const (e :('a, 'b) context) = !t1 t2. e t1 = e t2
+End
+
+Theorem WG_CONST :
+    !e. CCS_const e ==> WG e
+Proof
+    RW_TAC std_ss [CCS_const_def]
+ >> Know `e = (\t. e nil)` >- fs [FUN_EQ_THM]
+ >> Rewr' >> REWRITE_TAC [WG2]
+QED
+
+Theorem NO_WG8 :
+    !e X. ~CCS_const e ==> ~WG (\t. rec X (e t))
+Proof
+    rpt GEN_TAC >> ONCE_REWRITE_TAC [WG_cases]
+ >> fs [FUN_EQ_THM, CCS_const_def]
+ >> rpt STRIP_TAC
+ >> Cases_on `p` >> fs [FUN_EQ_THM]
+ >> METIS_TAC []
+QED
+
+Theorem WG8_IMP_CONST :
+    !e X. WG (\t. rec X (e t)) ==> CCS_const e
+Proof
+    METIS_TAC [NO_WG8]
 QED
 
 Theorem WG4_backward :
